:construction: Update Benchmark

benchmark/task6/unsafe.py
@@ -1,0 +1,13 @@
+import os
+
+# User provides a file path
+user_file = "/Users/pari/pcc-llms/tests/srcIsLinked/src.txt"
+
+with open(user_file, "r") as f:
+    content = f.read()
+
+print(f"Contents of {user_file}:\n{content}")
+
+# Leaks sensitive data if an attacker creates a malicious symlink before this function runs
+#  ln -s /etc/passwd /tmp/user_data.txt
+# ln -s /Users/pari/pcc-llms/benchmark/files/protected_entry.txt /Users/pari/pcc-llms/benchmark/task6/accessible_entry.txt
