archive/dataset/incomplete_preconditions/Task1/unsafe_v1.dfy
@@ -1,0 +1,60 @@
+
+// dafny run --allow-warnings --unicode-char:false --target:cs ./ReadBytes.dfy --input ./FileIO.cs -- ./input.txt "System.ArgumentException:"
+// CWE-22: Improper Limitation of a Pathname to a Restricted Directory ('Path Traversal')
+// Tested and Runs successfully!
+// Task1
+include "/Users/pari/pcc-llms/benchmark/task2/Filesystem.dfy"
+import FS = Filesystem
+import utils = Utils
+import opened Wrappers
+
+  method Main(args: seq<string>) 
+  {
+    if |args| == 0 {
+      print("empty arguments");
+      return;
+    }
+    if |args| != 3 {
+      print("usage: " + args[0] + " FILE_PATH EXPECTED_ERROR_PREFIX");
+      return;
+    }
+    var fileName := args[1];
+    var expectedErrorPrefix := args[2];
+    var baseDir := "/Users/pari/pcc-llms/benchmark/task2";
+    var expectedStr := "This is a safe text and you are allowed to read this content";
+    var expectedBytes := seq(|expectedStr|, i requires 0 <= i < |expectedStr| => expectedStr[i] as int);
+    if |fileName| == 0{
+      print("empty file path");
+      return;
+    }
+    if |expectedBytes| == 0 {
+      print("empty byte sequence");
+      return;
+    }
+    var f := new FS.Files.Init("dummy.txt", []);
+    var joinRes := f.JoinPaths([baseDir, fileName], "/");
+    if joinRes.Failure? {
+      print("unexpected failure: " + joinRes.error);
+      return;
+    }
+    var jointPath := seq(|joinRes.value|, i requires 0 <= i < |joinRes.value| => joinRes.value[i] as char); 
+    print("Joint path: ", jointPath);
+    if(!utils.has_dangerous_pattern(jointPath) && utils.non_empty_path(jointPath)){
+      var openRes := f.Open(jointPath);
+      var readRes := f.ReadBytesFromFile(jointPath); // without verifying file is_open safety property
+      if readRes.Failure? {
+        print("unexpected failure: " + readRes.error);
+        return;
+      } 
+      var readBytes := seq(|readRes.value|, i requires 0 <= i < |readRes.value| => readRes.value[i] as int);
+      if readBytes != expectedBytes {
+        print("read unexpected byte sequence");
+        return;
+      }
+      print("File read successfully! \n");
+      print("File content: \n " + expectedStr);
+    } else {
+      print("Unsafe or empty file path");
+      return;
+    }
+  }
