archive/dataset/incomplete_preconditions/Task3/unsafe_v4.dfy
@@ -1,0 +1,59 @@
+
+  // dafny run --allow-warnings --unicode-char:false --target:cs ./ReadBytes.dfy --input ./FileIO.cs -- ./input.txt "System.ArgumentException:"
+  // CWE-23 to cwe-29: Relative Path Traversal
+  // Tested and Runs successfully!
+
+  // Covers CWE-23 to CWE-29
+  include "/Users/pari/pcc-llms/benchmark/task3/Filesystem.dfy"
+  import FS = Filesystem
+  import utils = Utils
+  import strConverter = AsciiConverter
+  import opened Wrappers
+  method Main(args: seq<string>) 
+  {
+    if |args| == 0 {
+      print("empty arguments");
+      return;
+    }
+    if |args| != 4 {
+      print("usage: " + args[0] + " FILE_PATH EXPECTED_ERROR_PREFIX");
+      return;
+    }
+    var filePath := args[1];
+    var contentStr := args[2];
+    var expectedErrorPrefix := args[3];
+
+    var baseDir := "/Users/pari/pcc-llms/benchmark/task3";
+    var f := new FS.Files.Init("dummy.txt", []);
+    var joinRes := f.JoinPaths([baseDir, filePath], "/");
+    if joinRes.Failure? {
+      print("unexpected failure: " + joinRes.error);
+      return;
+    }
+    if !(utils.non_empty_string(contentStr)) {
+      print ("Empty string!\n");
+      return;
+    }
+    var jointPath := seq(|joinRes.value|, i requires 0 <= i < |joinRes.value| => joinRes.value[i] as char); 
+    var bytes :seq<bv8> := strConverter.strToBytes(contentStr); // Without verifying content characters
+    print("Joint path: \n", jointPath + "\n");
+    if (utils.has_backslash_dot_dot(jointPath) || utils.has_dot_dot_slash(jointPath)
+      || utils.has_dot_dot_backslash(jointPath) || utils.has_slash_dot_dot(jointPath) || 
+      !utils.non_empty_path(jointPath))
+      {
+        print("Invalid path! " + jointPath);
+        return;
+        } else {
+        var openRes := f.Open(jointPath);
+        if openRes.Failure? {
+          print ("unexpected error: \n" + openRes.error);
+          return;
+        }
+        var writeRes := f.WriteBytesToFile(jointPath, bytes);
+        if writeRes.Failure? {
+          print("unexpected failure writing to output_plain: \n" + writeRes.error);
+          return;
+        }
+        print("Write to the input file " + filePath + " was successfully! \n");
+    }  
+  }
