benchmark/task1/unsafe_v2.dfy
@@ -1,53 +1,32 @@
 
-// dafny run --allow-warnings --unicode-char:false --target:cs ./ReadBytes.dfy --input ./FileIO.cs -- ./input.txt "System.ArgumentException:"
 // CWE-22: Improper Limitation of a Pathname to a Restricted Directory ('Path Traversal')
-// Tested and Runs successfully!
+// dafny run --allow-warnings --unicode-char:false --target:cs absolute_path_to_dafny_file --input absolute_path_to_Filesystem.cs -- absolute_path_to_input_text_file "System.ArgumentException:"
+// Using any input file with path traversal pattern cause an error
 
-
-include "/Users/pari/pcc-llms/benchmark/task1/Filesystem.dfy"
+include "/Users/pari/pcc-llms/benchmark/Task1/Filesystem.dfy"
 import FS = Filesystem
 import utils = Utils
 import opened Wrappers
 
   method Main(args: seq<string>) 
   {
-    if |args| == 0 {
-      print("empty arguments");
-      return;
-    }
-    if |args| != 3 {
-      print("usage: " + args[0] + " FILE_PATH EXPECTED_ERROR_PREFIX");
-      return;
-    }
+    expect |args| > 0;
+    expect |args| == 3, "usage: " + args[0] + " FILE_PATH EXPECTED_ERROR_PREFIX";
     var filePath := args[1];
     var expectedErrorPrefix := args[2];
-    var expectedStr := "This is a safe text and you are allowed to read this content";
+    var expectedStr := "Hello!\nThis is a safe text and you are allowed to read this content\n";
     var expectedBytes := seq(|expectedStr|, i requires 0 <= i < |expectedStr| => expectedStr[i] as Utils.byte);
-    if |filePath| == 0{
-      print("empty file path");
-      return;
-    }
-    if |expectedBytes| == 0 {
-      print("empty byte sequence");
-      return;
-    }
+     expect |expectedBytes| > 0, "empty byte sequence";
+    expect |filePath| > 0, "empty file path";
     var f := new FS.Files.Init(filePath, expectedBytes);
-    print("Joint path: ", filePath);
-    var openRes := f.Open(filePath); // without verifying non-empty name string and dangerous pattern
-    if openRes.Failure? {
-      print("unexpected error: ", openRes.error);
-      return;
-    }
+    print("file path: ", filePath);
+    // {missing_specs}
+    var openRes := f.Open(filePath);
+    expect openRes.Success?, "unexpected error: " + openRes.error;
     var readRes := f.ReadBytesFromFile(filePath);
-    if readRes.Failure? {
-      print("unexpected failure: ", readRes.error);
-      return;
-    }
+    expect readRes.Success?, "unexpected failure: " + readRes.error;
     var readBytes := seq(|readRes.value|, i requires 0 <= i < |readRes.value| => readRes.value[i] as Utils.byte);
-    if readBytes != expectedBytes {
-      print("read unexpected byte sequence");
-      return;
-    } 
+    expect readBytes == expectedBytes, "read unexpected byte sequence";
     print("File read successfully! \n");
     print("File content: \n " + expectedStr);
   }
