benchmark/task3/unsafe_v2.dfy
@@ -11,46 +11,26 @@ import strConverter = AsciiConverter
 import opened Wrappers
 method Main(args: seq<string>) 
 {
-  if |args| == 0 {
-  print("empty arguments");
-  return;
-  }
-  if |args| != 4 {
-    print("usage: " + args[0] + " FILE_PATH EXPECTED_ERROR_PREFIX");
-    return;
-  }
+  expect |args| > 0;
+  expect |args| == 4, "usage: " + args[0] + " FILE_PATH CONTENT EXPECTED_ERROR_PREFIX";
   var filePath := args[1];
   var contentStr := args[2];
   var expectedErrorPrefix := args[3];
-
   var baseDir := "/Users/pari/pcc-llms/benchmark/task3";
+  expect |filePath| > 0;
+  expect |contentStr| > 0;
   var f := new FS.Files.Init("dummy.txt", []);
   var joinRes := f.JoinPaths([baseDir, filePath], "/");
-  if joinRes.Failure? {
-    print("unexpected failure: " + joinRes.error);
-    return;
-  }
-  if !(utils.non_empty_string(contentStr)) {
-    print ("Empty string!\n");
-    return;
-  }
-
-  if !(utils.is_valid_content_str(contentStr)) {
-    print ("Invalid content string!\n" + contentStr);
-    return;
-  }
-    var jointPath := seq(|joinRes.value|, i requires 0 <= i < |joinRes.value| => joinRes.value[i] as char); 
-    var bytes :seq<bv8> := strConverter.strToBytes(contentStr);
-    print("Joint path: \n", jointPath + "\n");
-    var openRes := f.Open(jointPath); // Without verifying if path has ../ or ..\ or /../ or \.. patterns
-    if openRes.Failure? {
-      print ("unexpected error: \n" + openRes.error);
-      return;
-    }
-    var writeRes := f.WriteBytesToFile(jointPath, bytes);
-    if writeRes.Failure? {
-      print("unexpected failure writing to output_plain: \n" + writeRes.error);
-      return;
-    }
-    print("Write to the input file " + filePath + " was successfully! \n"); 
+  expect !joinRes.Failure?, "unexpected failure: " + joinRes.error;
+  expect utils.non_empty_string(contentStr), "Empty string!";
+  expect utils.is_valid_content_str(contentStr), "Invalid content string!";
+  var jointPath := seq(|joinRes.value|, i requires 0 <= i < |joinRes.value| => joinRes.value[i] as char); 
+  var bytes :seq<bv8> := strConverter.strToBytes(contentStr);
+  print("Joint path: \n", jointPath + "\n");
+  // {missing_specs}
+  var openRes := f.Open(jointPath);
+  expect !openRes.Failure?, "unexpected error: " + openRes.error;
+  var writeRes := f.WriteBytesToFile(jointPath, bytes);
+  expect writeRes.Success?, "unexpected failure writing to output_plain: " + writeRes.error;
+  print("Write to the input file " + filePath + " was successfully! \n");
 }
