benchmark/task5/safe_v2.dfy
@@ -1,29 +1,30 @@
 
 // dafny run --allow-warnings --unicode-char:false --target:cs ./ReadBytes.dfy --input ./FileIO.cs -- ./input.txt "System.ArgumentException:"
-// CWE-22: Improper Limitation of a Pathname to a Restricted Directory ('Path Traversal')
+// CWE-23 to cwe-29: Relative Path Traversal
 // Tested and Runs successfully!
-include "/Users/pari/pcc-llms/benchmark/task2/Filesystem.dfy"
+
+// Covers CWE-23 to CWE-29
+include "/Users/pari/pcc-llms/benchmark/task5/Filesystem.dfy"
 import FS = Filesystem
 import utils = Utils
 import opened Wrappers
-
   method Main(args: seq<string>) 
   {
     expect |args| > 0;
-    expect |args| == 3, "usage: " + args[0] + " FILE_PATH EXPECTED_ERROR_PREFIX";
-    var fileName := args[1];
+    expect |args| == 3, "usage: " + args[0] + " FILE_PATH CONTENT EXPECTED_ERROR_PREFIX";
+    var filePath := args[1];
     var expectedErrorPrefix := args[2];
-    var baseDir := "/Users/pari/pcc-llms/benchmark/CWE-22";
+    var baseDir := "/Users/pari/pcc-llms/benchmark/task5";
     var f := new FS.Files.Init("dummy.txt", []);
-    var joinRes := f.JoinPaths([baseDir, fileName], "/");
+    var joinRes := f.JoinPaths([baseDir, filePath], "/");
     expect joinRes.Success?, "unexpected failure: " + joinRes.error;
     var jointPath := seq(|joinRes.value|, i requires 0 <= i < |joinRes.value| => joinRes.value[i] as char); 
-    var expectedStr := "This is a safe text and you are allowed to read this content";
+    var expectedStr := "Hello!\nThis is a safe text and you are allowed to read this content\n";
     var expectedBytes := seq(|expectedStr|, i requires 0 <= i < |expectedStr| => expectedStr[i] as int);
-    expect |expectedBytes| > 0, "empty byte sequence";
-    expect |fileName| > 0, "empty file path";
     print("Joint path: ", jointPath);
-    var openRes := f.Open(jointPath); // Without verifying non-empty path string and dangerous pattern
+    var pathCheck := f.PathIsInsideBase(baseDir, jointPath);
+    expect (!utils.has_dot_dot_slash(jointPath) && utils.non_empty_path(jointPath) && pathCheck);
+    var openRes := f.Open(jointPath);
     expect openRes.Success?, "unexpected error: " + openRes.error;
     var readRes := f.ReadBytesFromFile(jointPath);
     expect readRes.Success?, "unexpected failure: " + readRes.error;
@@ -31,4 +32,5 @@ import opened Wrappers
     expect readBytes == expectedBytes, "read unexpected byte sequence";
     print("File read successfully! \n");
     print("File content: \n " + expectedStr);
+
   }
