benchmark/task5/unsafe_v1.dfy
@@ -1,45 +1,48 @@
 
 // dafny run --allow-warnings --unicode-char:false --target:cs ./ReadBytes.dfy --input ./FileIO.cs -- ./input.txt "System.ArgumentException:"
-//  CWE-23 to cwe-29: Relative Path Traversal
+// CWE-23 to cwe-29: Relative Path Traversal
 // Tested and Runs successfully!
 
+// Covers CWE-23 to CWE-29
 include "/Users/pari/pcc-llms/benchmark/task5/Filesystem.dfy"
 import FS = Filesystem
 import utils = Utils
 import opened Wrappers
   method Main(args: seq<string>) 
   {
-    expect |args| > 0;
-    expect |args| == 3, "usage: " + args[0] + " FILE_PATH EXPECTED_ERROR_PREFIX";
+    if |args| == 0 {
+      print("empty arguments");
+      return;
+    }
+    if |args| != 3 {
+      print("usage: " + args[0] + " FILE_PATH EXPECTED_ERROR_PREFIX");
+      return;
+    }
     var filePath := args[1];
     var expectedErrorPrefix := args[2];
-    var baseDir := "/Users/pari/pcc-llms/benchmark/CWE-23/dafny";
+    var baseDir := "/Users/pari/pcc-llms/benchmark/task5";
     var f := new FS.Files.Init("dummy.txt", []);
     var joinRes := f.JoinPaths([baseDir, filePath], "/");
+    if joinRes.Failure? {
+      print("unexpected failure: " + joinRes.error);
+      return;
+    }
     var jointPath := seq(|joinRes.value|, i requires 0 <= i < |joinRes.value| => joinRes.value[i] as char); 
     var expectedStr := "Hello!\nThis is a safe text and you are allowed to read this content\n";
     var expectedBytes := seq(|expectedStr|, i requires 0 <= i < |expectedStr| => expectedStr[i] as int);
     print("Joint path: ", jointPath);
-    if(!utils.has_backslash_dot_dot(jointPath) && !utils.has_dot_dot_slash(jointPath)
-    && !utils.has_dot_dot_backslash(jointPath) && !utils.has_slash_dot_dot(jointPath) && utils.non_empty_path(jointPath)){
-      var openRes := f.Open(jointPath);
-      if openRes.Failure? {
-        expect openRes.Success?, "unexpected error: " + openRes.error;
-        return;
-      }
-      var readRes := f.ReadBytesFromFile(jointPath);
-      if readRes.Failure? {
-        expect readRes.Success?, "unexpected failure: " + readRes.error;
-        var readResEmpty := f.ReadBytesFromFile("");
-        expect readResEmpty.Failure?, "unexpected success";
-        expect expectedErrorPrefix <= readResEmpty.error, "unexpected error message: " + readResEmpty.error;
-      } else {
-        var readBytes := seq(|readRes.value|, i requires 0 <= i < |readRes.value| => readRes.value[i] as int);
-        expect readBytes == expectedBytes, "read unexpected byte sequence";
-      } 
-      print("File read successfully! \n");
-      print("File content: \n " + expectedStr);
-      } else {
-        return;
-      }
+      // {missing_specs}
+    var openRes := f.Open(jointPath);
+    if openRes.Failure? {
+      print("unexpected error: " + openRes.error);
+      return;
+    }
+    var readRes := f.ReadBytesFromFile(jointPath);
+    if readRes.Failure? {
+      print("unexpected failure: " + readRes.error);
+      return;
+    }
+    var readBytes := seq(|readRes.value|, i requires 0 <= i < |readRes.value| => readRes.value[i] as int);
+    print("File read successfully! \n");
+    print("File content: \n " + expectedStr);
   }
