benchmark/task7/Filesystem.dfy
@@ -1,0 +1,194 @@
+/*******************************************************************************
+ *  Copyright by the contributors to the Dafny Project
+ *  SPDX-License-Identifier: MIT
+ *******************************************************************************/
+
+// RUN: %verify "%s"
+
+include "/Users/pari/pcc-llms/stdlib/Wrappers.dfy"
+include "/Users/pari/pcc-llms/stdlib/utils/Utils.dfy"
+
+/**
+  * This module provides basic file I/O operations: reading and writing bytes from/to a file.
+  * The provided API is intentionally limited in scope and will be expanded later.
+  *
+  * Where the API accepts file paths as strings, there are some limitations.
+  * File paths containing only ASCII characters work identically across languages and platforms;
+  * non-ASCII Unicode codepoints may cause different language- or platform-specific behavior.
+  *
+  * File path symbols including . and .. are allowed.
+  */
+
+module {:options "-functionSyntax:4"} Filesystem {
+  import opened Wrappers
+  import Utils
+  datatype Error =  Noent | Exist
+  datatype Ok<T> = Ok(v: T)
+
+
+  class Files {
+    var name: string
+    var contents: seq<Utils.byte>
+    ghost var is_open:bool // Ghost variable can only be used in the specifications
+    ghost var is_symbolic_link:bool
+
+    // constructor Init(){
+    //   is_open := false;
+    //   is_symbolic_link := false;
+    // }
+
+    
+    constructor Init (n: string, c: seq<Utils.byte>)
+      requires n != ""       // We can't create a file with an empty name
+      ensures name == n
+      ensures contents == c
+    {
+      name := n;
+      contents := c;
+      is_open := false;
+      is_symbolic_link := false;
+    }
+
+    method Size() returns (s: int)
+      ensures s == |contents|
+    {
+      s := |contents|;
+    }
+     /**
+    * Opens a file at the given path.
+    * Checks if the file exists and resolves its absolute path.
+    * Returns a `Result` containing a `FileHandle` on success or an error message on failure.
+    *
+    * NOTE: See the module description for limitations on the path argument.
+    */
+
+    // method fileExists(file: string) returns (res: Result<bool, string>)
+    // {
+    //   var isError, fileExists, errorMsg := INTERNAL_fileExists(file);
+    //   return if isError then Failure(errorMsg) else Success(fileExists);
+    // }
+ 
+    method Open(file: string) returns (res: Result<object, string>)
+      // requires is_open == false // If I use this precondition, I get an error when I use f.Open(filePath) in cwe-22-safe.dfy
+      modifies this
+      requires !Utils.has_dangerous_pattern(file)
+      requires Utils.non_empty_path(file)
+      ensures is_open == if res.Success? then true else false
+    {
+        var isError, fileStream, errorMsg := INTERNAL_Open(file);
+        is_open := if isError then false else true;
+        return if isError then Failure(errorMsg) else Success(fileStream);
+      
+    }
+    /*
+    * Public API
+    */
+
+    /**
+      * Attempts to read all bytes from the file at the given file path.
+      * If an error occurs, a `Result.Failure` value is returned containing an implementation-specific
+      * error message (which may also contain a stack trace).
+      *
+      * NOTE: See the module description for limitations on the path argument.
+      */
+    method ReadBytesFromFile(file: string) returns (res: Result<seq<bv8>, string>) 
+    //TODO: Add a precondition to check if the file exists
+    requires this.is_open == true
+    {
+      var isError, bytesRead, errorMsg := INTERNAL_ReadBytesFromFile(file);
+      return if isError then Failure(errorMsg) else Success(bytesRead);
+    }
+
+    /**
+      * Attempts to write the given bytes to the file at the given file path,
+      * creating nonexistent parent directories as necessary.
+      * If an error occurs, a `Result.Failure` value is returned containing an implementation-specific
+      * error message (which may also contain a stack trace).
+      *
+      * NOTE: See the module description for limitations on the path argument.
+      */
+    method WriteBytesToFile(file: string, bytes: seq<bv8>) returns (res: Result<(), string>)
+    requires this.is_open == true
+    {
+      var isError, errorMsg := INTERNAL_WriteBytesToFile(file, bytes);
+      return if isError then Failure(errorMsg) else Success(());
+    }
+
+
+    method IsLink(file: string) returns (res: Result<bool, string>) 
+    {
+      var isError, isLink, errorMsg := INTERNAL_IsLink(file);
+      if isError {
+        res := Failure(errorMsg);
+      } else {
+        res := Success(isLink);
+      }
+    }
+
+
+    method JoinPaths(paths: seq<string>, separator: string) returns (res: Result<string, string>) 
+    requires |separator| == 1
+    requires |paths| > 0
+    ensures res.Success? ==> Utils.non_empty_path(res.value) && !Utils.has_dangerous_pattern(res.value)
+    {
+      if |paths| == 0 || |separator| == 0 {
+        return Failure("Paths or separator cannot be empty.");
+      }
+
+      var combinedPath := "";
+      var i := 0;
+      while i < |paths|
+      invariant 0 <= i <= |paths| 
+      invariant |combinedPath| >= i  
+      decreases |paths| - i 
+      {
+        combinedPath := combinedPath + paths[i] + separator; 
+        i := i + 1;
+      }
+
+    if !Utils.non_empty_path(combinedPath) {
+      return Failure("Resulting path is empty.");
+    }
+    if Utils.has_dangerous_pattern(combinedPath) {
+      return Failure("Resulting path contains dangerous patterns.");
+    }
+
+      var isError, fullPath, errorMsg := INTERNAL_JoinPaths(paths, separator);
+      if !isError {
+        assert Utils.non_empty_path(fullPath);
+        assert !Utils.has_dangerous_pattern(fullPath);
+      }
+      var notValidPath := if fullPath != combinedPath then false else true;
+      return if (isError || notValidPath) then Failure(errorMsg) else Success(fullPath);
+    }
+    
+
+  }
+
+    method
+      {:extern "Filesystem.Files", "INTERNAL_Open"}
+    INTERNAL_Open(file: string)
+      returns (isError: bool, fs: object, errorMsg: string)
+
+
+    method
+      {:extern "Filesystem.Files", "INTERNAL_ReadBytesFromFile"}
+    INTERNAL_ReadBytesFromFile(file: string)
+      returns (isError: bool, bytesRead: seq<bv8>, errorMsg: string)
+
+    method
+      {:extern "Filesystem.Files", "INTERNAL_WriteBytesToFile"}
+    INTERNAL_WriteBytesToFile(file: string, bytes: seq<bv8>)
+      returns (isError: bool, errorMsg: string)
+
+    method
+    {:extern "Filesystem.Files", "INTERNAL_IsLink"}
+    INTERNAL_IsLink(file: string)
+    returns ( isError: bool, isLink: bool, errorMsg: string)
+
+    method
+      {:extern "Filesystem.Files", "INTERNAL_JoinPaths"}
+    INTERNAL_JoinPaths(paths: seq<string>, separator: string)
+    returns (isError: bool, fullPath: string, errorMsg: string)
+    ensures !isError ==> Utils.non_empty_path(fullPath) && !Utils.has_dangerous_pattern(fullPath)
+}
